Add proofs for Thermopot

case-studies/thermopot/Requirements.thy
@@ -9,11 +9,11 @@ getVarBool s2 lid' = LOCKED')"
 
 definition R2 where "R2 s \<equiv> toEnvP s \<and>
 (\<forall> s1 s2. substate s1 s2 \<and> substate s2 s \<and> toEnvP s1 \<and> toEnvP s2 \<and> toEnvNum s1 s2 = 1 \<and>
-getVarBool s1 maintainingMode' \<and> getVarInt s1 temperature' \<ge> getVarInt s1 selectedTemp' \<longrightarrow> getVarBool s1 heater' = False)"
+getVarBool s1 maintainingMode' \<and> \<not> (getVarBool s2 boilingButton' = PRESSED') \<and> getVarInt s2 temperature' \<ge> getVarInt s2 selectedTemp' \<longrightarrow> getVarBool s2 heater' = False)"
 
 definition R3 where "R3 s \<equiv> toEnvP s \<and>
 (\<forall> s1 s2. substate s1 s2 \<and> substate s2 s \<and> toEnvP s1 \<and> toEnvP s2 \<and> toEnvNum s1 s2 = 1 \<and>
-getVarBool s1 maintainingMode' \<and> getVarInt s2 temperature' < getVarInt s2 selectedTemp' - 5 \<longrightarrow>
+getVarBool s1 maintainingMode' \<and> \<not> getVarBool s2 boilingButton' = PRESSED' \<and> getVarInt s2 temperature' < getVarInt s2 selectedTemp' - 5 \<longrightarrow>
 getVarBool s2 heater' = True)"
 
 definition R4 where "R4 s \<equiv> toEnvP s \<and>
