case-studies/thermopot/ExtraInv.thy
@@ -1,0 +1,26 @@
+theory ExtraInv
+  imports Requirements VCTheoryLemmas
+begin
+
+definition extraInv where "extraInv s \<equiv> toEnvP s \<and>
+(\<forall> s1. toEnvP s1 \<and> substate s1 s \<and> getPstate s1 HeaterController' = HeaterController'begin' \<longrightarrow> 
+getVarBool s1 boilingMode' = False \<and> getVarBool s1 maintainingMode' = False \<and> getVarBool s1 heater' = False) \<and>
+(\<forall> s1. toEnvP s1 \<and> substate s1 s \<and> getPstate s1 HeaterController' = HeaterController'heating' \<longrightarrow>
+ getVarBool s1 boilingMode' = True \<and> getVarBool s1 maintainingMode' = False) \<and>
+(\<forall> s1. toEnvP s1 \<and> substate s1 s \<and> getPstate s1 HeaterController' =  HeaterController'maintaining' \<longrightarrow>
+getVarBool s1 boilingMode' = False \<and> getVarBool s1 maintainingMode' = True) \<and>
+(\<forall> s1. toEnvP s1 \<and> substate s1 s \<and> getPstate s1 HeaterController' = STOP \<longrightarrow> 
+getVarBool s1 boilingMode' = False \<and> getVarBool s1 maintainingMode' = False \<and> getVarBool s1 heater' = False) \<and>
+(\<forall> s1. toEnvP s1 \<and> substate s1 s \<longrightarrow> (getPstate s1 Init' = Init'begin' \<longleftrightarrow> toEnvNum emptyState s1 = 1)) \<and>
+(\<forall> s1. toEnvP s1 \<and> substate s1 s \<longrightarrow> (getPstate s1 HeaterController' = STOP \<longleftrightarrow> toEnvNum emptyState s1 = 1)) \<and>
+(\<forall> s1. toEnvP s1 \<and> substate s1 s \<longrightarrow> (getPstate s1 TempSelection' = STOP \<longleftrightarrow> toEnvNum emptyState s1 = 1)) \<and>
+(\<forall> s1. toEnvP s1 \<and> substate s1 s \<longrightarrow>
+ getPstate s1 HeaterController' \<in> {HeaterController'begin', HeaterController'heating', HeaterController'maintaining', STOP})\<and>
+(\<forall> s1. toEnvP s1 \<and> substate s1 s \<longrightarrow> getPstate s1 TempSelection' \<in> {TempSelection'tempSelection', STOP}) "
+
+theorem extra_1: "VC1 extraInv s0"
+  apply(unfold VC1_def extraInv_def)
+  by simp
+
+
+end
