case-studies/thermopot/ExtraInv_VC62.thy
@@ -1,0 +1,37 @@
+theory ExtraInv_VC62
+  imports ExtraInv
+begin
+
+theorem extra_62: "VC62 extraInv env s0 temperature_value button1_value button2_value button3_value boilingButton_value "
+  apply(unfold VC62_def extraInv_def)
+  apply(rule impI)
+  apply(erule conjE)
+  apply(erule conjE)
+  subgoal premises prems
+    apply(insert prems(2))
+    apply((erule conjE)+)
+    subgoal premises ei
+      apply(insert ei(1))
+      apply(rule conjI)
+       apply simp
+      apply(rule conjI)
+      using ei(2) apply simp
+      apply(rule conjI)
+      using ei(3) ei(2) prems(1) apply simp
+      apply(rule conjI)
+      using ei(4) apply simp
+      apply(rule conjI)
+      using ei(5) apply simp
+      apply(rule conjI)
+      using ei(6) prems(1) toEnvP_imp_gtime_gt_0 apply simp
+      apply(rule conjI)
+      using ei(7) toEnvP_imp_gtime_gt_0 apply simp
+      apply(rule conjI)
+      using ei(8) prems(1) toEnvP_imp_gtime_gt_0 apply simp
+      apply(rule conjI)
+      using ei(9) apply simp
+      using ei(10) by simp
+    done
+  done
+
+end
