case-studies/thermopot/Proof_R1_VC62.thy
@@ -1,0 +1,29 @@
+theory Proof_R1_VC62
+  imports Proofs1 ExtraInv_VC62
+begin
+
+theorem proof_1_62: "VC62 inv1 env s0 temperature_value button1_value button2_value button3_value boilingButton_value "
+  apply(unfold VC62_def inv1_def R1_def)
+  apply(rule impI)
+  apply(rule conjI)
+   apply(rule conjI)
+    apply simp
+  apply(unfold extraInv_def)[1]
+   apply(erule conjE)
+   apply(erule conjE)
+  subgoal premises prems
+    apply(insert prems(2))
+    apply(erule conjE)
+    apply((erule conjE)+)
+    subgoal premises invs0
+      apply((rule allI)+)
+      apply(rule impI)
+      apply(simp split: if_splits)
+      using prems(1) apply simp
+      using invs0
+       apply (metis substate_toEnvNum_id) 
+      using invs0(1,2) by auto
+    done
+  using extra_62 by (auto simp add: VC62_def)
+
+end
