case-studies/thermopot/Proof_R2_VC65.thy
@@ -1,0 +1,29 @@
+theory Proof_R2_VC65
+  imports Proofs2 ExtraInv_VC65
+begin
+
+theorem proof_2_65: "VC65 inv2 env s0 temperature_value button1_value button2_value button3_value boilingButton_value "
+  apply(unfold VC65_def inv2_def R2_def)
+  apply(rule impI)
+  apply(rule conjI)
+   apply(rule conjI)
+    apply simp
+  apply(unfold extraInv_def)[1]
+   apply(erule conjE)
+   apply(erule conjE)
+  subgoal premises prems
+    apply(insert prems(2))
+    apply(erule conjE)
+    apply((erule conjE)+)
+    subgoal premises invs0
+      apply((rule allI)+)
+      apply(rule impI)
+      apply(simp split: if_splits)
+      using prems(1) apply simp
+      using invs0
+       apply (metis substate_toEnvNum_id)
+      using invs0(2) by auto
+    done
+  using extra_65 by(auto simp add: VC65_def)
+
+end
