case-studies/thermopot/Proof_R5_VC3.thy
@@ -1,0 +1,29 @@
+theory Proof_R5_VC3
+  imports Proofs5 ExtraInv_VC3
+begin
+
+theorem proof_5_3: "VC3 inv5 env s0 temperature_value button1_value button2_value button3_value boilingButton_value "
+  apply(unfold VC3_def inv5_def R5_def)
+  apply(rule impI)
+  apply(rule conjI)
+   apply(rule conjI)
+    apply simp
+  apply(unfold extraInv_def)[1]
+   apply(erule conjE)
+   apply(erule conjE)
+  subgoal premises prems
+    apply(insert prems(2))
+    apply(erule conjE)
+    apply((erule conjE)+)
+    subgoal premises invs0
+      apply((rule allI)+)
+      apply(rule impI)
+      apply(simp split: if_splits)
+      using prems(1) apply simp
+      using invs0
+       apply (metis substate_toEnvNum_id)
+      using invs0(2) by auto
+    done
+  using extra_3 by(auto simp add: VC3_def)
+
+end
