case-studies/thermopot/Proofs1.thy
@@ -1,0 +1,19 @@
+theory Proofs1
+  imports ExtraInv
+begin
+
+definition inv1 where "inv1 s \<equiv> R1 s \<and> extraInv s"
+
+theorem proof_1_1: "VC1 inv1 s0"
+  apply(unfold VC1_def inv1_def R1_def extraInv_def)
+  by simp
+
+theorem proof_1_64: "VC64 R1 env s0 temperature_value button1_value button2_value button3_value boilingButton_value "
+  apply(unfold VC64_def  R1_def extraInv_def)
+  by auto
+
+theorem proof_1_65: "VC65 R1 env s0 temperature_value button1_value button2_value button3_value boilingButton_value "
+  apply(unfold VC65_def  R1_def extraInv_def)
+  by auto
+
+end
