case-studies/thermopot/Proofs2.thy
@@ -1,0 +1,35 @@
+theory Proofs2
+  imports ExtraInv
+begin
+
+definition inv2 where "inv2 s \<equiv> R2 s \<and> extraInv s"
+
+theorem proof_2_1: "VC1 inv2 s0"
+  apply(unfold VC1_def inv2_def R2_def extraInv_def)
+  by simp
+
+theorem proof_2_62: "VC62 R2 env s0 temperature_value button1_value button2_value button3_value boilingButton_value "
+  apply(unfold VC62_def inv2_def R2_def extraInv_def)
+  by auto
+
+theorem proof_2_64: "VC64 R2 env s0 temperature_value button1_value button2_value button3_value boilingButton_value "
+  apply(unfold VC64_def inv2_def R2_def extraInv_def)
+  by auto
+
+theorem proof_2_66: "VC66 R2 env s0 temperature_value button1_value button2_value button3_value boilingButton_value "
+  apply(unfold VC66_def inv2_def R2_def extraInv_def)
+  by auto
+
+theorem proof_2_67: "VC67 R2 env s0 temperature_value button1_value button2_value button3_value boilingButton_value "
+  apply(unfold VC67_def inv2_def R2_def extraInv_def)
+  by auto
+
+theorem proof_2_68: "VC68 R2 env s0 temperature_value button1_value button2_value button3_value boilingButton_value "
+  apply(unfold VC68_def inv2_def R2_def extraInv_def)
+  by auto
+
+theorem proof_2_69: "VC69 R2 env s0 temperature_value button1_value button2_value button3_value boilingButton_value "
+  apply(unfold VC69_def inv2_def R2_def extraInv_def)
+  by auto
+
+end
