case-studies/thermopot/Proofs5.thy
@@ -1,0 +1,19 @@
+theory Proofs5
+  imports ExtraInv
+begin
+
+definition inv5 where "inv5 s \<equiv> R5 s \<and> extraInv s"
+
+theorem proof_5_1: "VC1 inv5 s0"
+  apply(unfold VC1_def inv5_def R5_def extraInv_def)
+  by auto
+
+theorem proof_5_64: "VC64 R5 env s0 temperature_value button1_value button2_value button3_value boilingButton_value "
+  apply(unfold VC64_def inv5_def R5_def extraInv_def)
+  by auto
+
+theorem proof_5_67: "VC67 R5 env s0 temperature_value button1_value button2_value button3_value boilingButton_value "
+  apply(unfold VC67_def inv5_def R5_def extraInv_def)
+  by auto
+
+end
